Given_Clause_Loops/Fair_Zipperposition_Loop.thy
@@ -35,10 +35,10 @@ locale fair_discount_loop =
     Equiv_F :: "'f \<Rightarrow> 'f \<Rightarrow> bool" (infix \<open>\<doteq>\<close> 50) and
     Prec_F :: "'f \<Rightarrow> 'f \<Rightarrow> bool" (infix \<open>\<prec>\<cdot>\<close> 50) and
     t_empty :: "'t" and
-    t_select :: "'t \<Rightarrow> 'f" and
-    t_add :: "'f \<Rightarrow> 't \<Rightarrow> 't" and
-    t_remove :: "'f \<Rightarrow> 't \<Rightarrow> 't" and
-    t_felems :: "'t \<Rightarrow> 'f fset" and
+    t_select :: "'t \<Rightarrow> 'f inference llist" and
+    t_add :: "'f inference llist \<Rightarrow> 't \<Rightarrow> 't" and
+    t_remove :: "'f inference llist \<Rightarrow> 't \<Rightarrow> 't" and
+    t_felems :: "'t \<Rightarrow> 'f inference llist fset" and
     p_empty :: "'p" and
     p_select :: "'p \<Rightarrow> 'f" and
     p_add :: "'f \<Rightarrow> 'p \<Rightarrow> 'p" and
@@ -51,6 +51,86 @@ locale fair_discount_loop =
     transp_Prec_S: "transp (\<prec>S)"
 begin
 
+lemma trans_Prec_S: "trans {(x, y). x \<prec>S y}"
+  using transp_Prec_S transp_trans by blast
+
+lemma irreflp_Prec_S: "irreflp (\<prec>S)"
+  using minimal_element.wf wfP_imp_irreflp wf_Prec_S wfp_on_UNIV by blast
+
+lemma irrefl_Prec_S: "irrefl {(x, y). x \<prec>S y}"
+  by (metis CollectD case_prod_conv irrefl_def irreflp_Prec_S irreflp_def)
+
+
+subsection \<open>Definition and Lemmas\<close>
+
+abbreviation todo_of :: "('t, 'p, 'f) fair_ZL_state \<Rightarrow> 't" where
+  "todo_of St \<equiv> fst St"
+abbreviation passive_of :: "('t, 'p, 'f) fair_ZL_state \<Rightarrow> 'p" where
+  "passive_of St \<equiv> fst (snd St)"
+abbreviation yy_of :: "('t, 'p, 'f) fair_ZL_state \<Rightarrow> 'f option" where
+  "yy_of St \<equiv> fst (snd (snd St))"
+abbreviation active_of :: "('t, 'p, 'f) fair_ZL_state \<Rightarrow> 'f fset" where
+  "active_of St \<equiv> snd (snd (snd St))"
+
+abbreviation formulas_of :: "('t, 'p, 'f) fair_ZL_state \<Rightarrow> 'f set" where
+  "formulas_of St \<equiv> passive.elems (passive_of St) \<union> set_option (yy_of St) \<union> fset (active_of St)"
+
+fun zl_fstate :: "('t, 'p, 'f) fair_ZL_state \<Rightarrow> 'f inference set \<times> ('f \<times> DL_label) set" where
+  "zl_fstate (T, P, Y, A) = zl_state (todo.elems T, passive.elems P, set_option Y, fset A)"
+
+lemma zl_fstate_alt_def:
+  "zl_fstate St = zl_state (todo.elems (fst St), passive.elems (fst (snd St)),
+     set_option (fst (snd (snd St))), fset (snd (snd (snd St))))"
+  by (cases St) auto
+
+definition
+  Liminf_zl_fstate :: "('t, 'p, 'f) fair_ZL_state llist \<Rightarrow> 'f set \<times> 'f set \<times> 'f set"
+where
+  "Liminf_zl_fstate Sts =
+   (Liminf_llist (lmap (passive.elems \<circ> passive_of) Sts),
+    Liminf_llist (lmap (set_option \<circ> yy_of) Sts),
+    Liminf_llist (lmap (fset \<circ> active_of) Sts))"
+
+lemma Liminf_fstate_commute:
+  "Liminf_llist (lmap (snd \<circ> zl_fstate) Sts) = labeled_formulas_of (Liminf_zl_fstate Sts)"
+proof -
+  have "Liminf_llist (lmap (snd \<circ> zl_fstate) Sts) =
+    (\<lambda>C. (C, Passive)) ` Liminf_llist (lmap (passive.elems \<circ> passive_of) Sts) \<union>
+    (\<lambda>C. (C, YY)) ` Liminf_llist (lmap (set_option \<circ> yy_of) Sts) \<union>
+    (\<lambda>C. (C, Active)) ` Liminf_llist (lmap (fset \<circ> active_of) Sts)"
+    unfolding zl_fstate_alt_def zl_state_alt_def
+    apply simp
+    apply (subst Liminf_llist_lmap_union, fast)+
+    apply (subst Liminf_llist_lmap_image, simp add: inj_on_convol_ident)+
+    by auto
+ thus ?thesis
+   unfolding Liminf_zl_fstate_def by fastforce
+qed
+
+fun formulas_union :: "'f set \<times> 'f set \<times> 'f set \<Rightarrow> 'f set" where
+  "formulas_union (P, Y, A) = P \<union> Y \<union> A"
+
+inductive
+  fair_ZL :: "('t, 'p, 'f) fair_ZL_state \<Rightarrow> ('t, 'p, 'f) fair_ZL_state \<Rightarrow> bool"
+  (infix "\<leadsto>ZLf" 50)
+where
+  compute_infer: "T \<noteq> t_empty \<Longrightarrow> t_select T = LCons \<iota>0 \<iota>s \<Longrightarrow>
+    \<iota>0 \<in> no_labels.Red_I (fset A \<union> {C}) \<Longrightarrow>
+    (T, P, None, A) \<leadsto>ZLf (t_add \<iota>s (t_remove (t_select T) T), p_add C P, None, A)"
+| choose_p: "P \<noteq> p_empty \<Longrightarrow>
+    (T, P, None, A) \<leadsto>ZLf (T, p_remove (p_select P) P, Some (p_select P), A)"
+| delete_fwd: "C \<in> no_labels.Red_F (fset A) \<or> (\<exists>C' \<in> fset A. C' \<preceq>\<cdot> C) \<Longrightarrow>
+    (T, P, Some C, A) \<leadsto>ZLf (T, P, None, A)"
+| simplify_fwd: "C' \<prec>S C \<Longrightarrow> C \<in> no_labels.Red_F (fset A \<union> {C'}) \<Longrightarrow>
+    (T, P, Some C, A) \<leadsto>ZLf (T, P, Some C', A)"
+| delete_bwd: "C' |\<notin>| A \<Longrightarrow> C' \<in> no_labels.Red_F {C} \<or> C' \<cdot>\<succ> C \<Longrightarrow>
+    (T, P, Some C, A |\<union>| {|C'|}) \<leadsto>ZLf (T, P, Some C, A)"
+| simplify_bwd: "C' |\<notin>| A \<Longrightarrow> C'' \<prec>S C' \<Longrightarrow> C' \<in> no_labels.Red_F {C, C''} \<Longrightarrow>
+    (T, P, Some C, A |\<union>| {|C'|}) \<leadsto>ZLf (T, p_add C'' P, Some C, A)"
+| schedule_infer: "flat_inferences_of (set \<iota>ss) = no_labels.Inf_between (fset A) {C} \<Longrightarrow>
+    (T, P, Some C, A) \<leadsto>ZLf (fold t_add \<iota>ss T, P, None, A |\<union>| {|C|})"
+| delete_orphan_infers: "\<iota>s \<in> todo.elems T \<Longrightarrow> lset \<iota>s \<inter> no_labels.Inf_from (fset A) = {} \<Longrightarrow>
+    (T, P, Y, A) \<leadsto>ZLf (t_remove \<iota>s T, P, Y, A)"
 
 end
 
